LeanNanoLlvm.lean
@@ -2,5 +2,6 @@
 -- Import modules here that should be built as part of the library.
 import LeanNanoLlvm.AST
 import LeanNanoLlvm.Semantics
+import LeanNanoLlvm.Refinement
 import LeanNanoLlvm.Tactic
 import LeanNanoLlvm.Util
