LeanNanoLlvm/Refinement/Refinement.lean
@@ -1,0 +1,75 @@
+/-
+Released under Apache 2.0 license as described in the LICENSE of Lean-MLIR.
+
+https://github.com/opencompl/lean-mlir
+-/
+
+import LeanNanoLlvm.Tactic
+import Mathlib.Order.Defs.Unbundled
+
+/--
+The notation typeclass for heterogenous refinement relations.
+This enables the notation `a ⊑ b`, where `a : α` and `b : β`.
+
+NOTE: This typeclass is not intended for dialect implementors. Please implement
+`DialectRefinement` instead, from which appropriate `HRefinement` instances will
+be inferred.
+-/
+class HRefinement (α β : Type) where
+  /--
+  We say that `a` is refined by `b`, written as `a ⊑ b`, when
+  every observable behaviour of `b` is allowed by `a`.
+
+  Note that this notation is driven by a typeclass, thus the exact meaning
+  is type-dependent.
+  -/
+  IsRefinedBy : α → β → Prop
+
+@[inherit_doc] infix:50 " ⊑ "  => HRefinement.IsRefinedBy
+
+/--
+The homogenous version of `HRefinement`.
+This enables the notation `a ⊑ b`, where `a, b : α`.
+
+NOTE: This typeclass is not intended for dialect implementors. Please implement
+`DialectRefinement` instead.
+-/
+class Refinement (α : Type) where
+  IsRefinedBy : α → α → Prop
+
+instance instHRefinementOfRefinement [Refinement α] : HRefinement α α where
+  IsRefinedBy := Refinement.IsRefinedBy
+
+@[simp_denote]
+def Refinement.ofHRefinement (inst : HRefinement α α) : Refinement α where
+  IsRefinedBy x y := x ⊑ y
+
+section OfEq
+
+/-- Equality induces a trivial (homogenous) refinement relation on any type `α`. -/
+def Refinement.ofEq : Refinement α where
+  IsRefinedBy := Eq
+
+instance (priority := low) :
+    Std.Refl (HRefinement.IsRefinedBy (self := @instHRefinementOfRefinement α .ofEq)) where
+  refl _ := rfl
+instance (priority := low) :
+    IsTrans α (HRefinement.IsRefinedBy (self := @instHRefinementOfRefinement α .ofEq)) where
+  trans _ _ _ := Eq.trans
+instance (priority := low) [DecidableEq α] :
+    Decidable (HRefinement.IsRefinedBy (self := @instHRefinementOfRefinement α .ofEq) x y) :=
+  decidable_of_iff (x = y) (by rfl)
+
+end OfEq
+
+/-! ### Id Refinement -/
+namespace Id
+variable {α β} [inst : HRefinement α β]
+
+instance instRefinement : HRefinement (Id α) (Id β) := inst
+
+@[simp_denote (high)] -- high priority so that this is tried before the `reduceIsRefinedBy` simproc
+theorem pure_isRefinedBy_pure (x : α) (y : β) :
+  (pure x : Id _) ⊑ (pure y : Id _) ↔ x ⊑ y := by rfl
+
+end Id
